@prefix owl: <http://www.w3.org/2002/07/owl#> .
@prefix rdfs: <http://www.w3.org/2000/01/rdf-schema#> .
@prefix skos: <http://www.w3.org/2004/02/skos/core#> .
@prefix foaf: <http://xmlns.com/foaf/0.1/> .
@prefix dct: <http://purl.org/dc/terms/> .
@prefix cc: <http://creativecommons.org/ns#> .
@prefix era-op-types: <http://era.europa.eu/concepts/op-types#> .
@prefix era-vehicles: <http://era.europa.eu/concepts/vehicles#> .
@prefix era-manufacturers:  <http://era.europa.eu/concepts/manufacturers#> .
@prefix era-lc: <http://era.europa.eu/concepts/load-capabilities#> .
@prefix era-gaugings: <http://era.europa.eu/concepts/gaugings#> .
@prefix era-tds: <http://era.europa.eu/concepts/train-detection#> .
@prefix era-ftds: <http://era.europa.eu/concepts/french-train-detection#> .
@prefix era-am: <http://era.europa.eu/concepts/axle-monitoring#> .
@prefix era-tc: <http://era.europa.eu/concepts/thermal-capacity#> .
@prefix era-ic: <http://era.europa.eu/concepts/ice-conditions#> .
@prefix era-cls: <http://era.europa.eu/concepts/contact-line-systems#> .
@prefix era-rs-fire: <http://era.europa.eu/concepts/rs-fire#> .


#################################################################
#
#    Abstract Concepts
#
#################################################################

era-op-types:OperationalPointType a owl:Class ; # Concepts of this class are dynamically genereated at mapping time
    rdfs:subClassOf skos:Concept ;
    rdfs:label "Operational Point Type"@en ;
    rdfs:comment "Abstract class representing the different existing types of Operational Points"@en .

era-vehicles:Category a owl:Class ;
    rdfs:subClassOf skos:Concept ;
    rdfs:label "Vehicle Category"@en ;
    rdfs:comment "Abstract class representing vehicle categories"@en .

era-vehicles:SubCategory a owl:Class ;
    rdfs:subClassOf skos:Concept ;
    rdfs:label "Vehicle Sub Category"@en ;
    rdfs:comment "Abstract class representing vehicle sub categories"@en .

era-manufacturers:Manufacturer a owl:Class ; # Concepts of this class are dynamically genereated at mapping time
    rdfs:subClassOf skos:Concept ;
    rdfs:label "Manufacturer"@en ;
    rdfs:comment "Abstract class representing vehicle manufacturer companies"@en .

era-lc:LoadCapability a owl:Class ; # Concepts of this class are dynamically genereated at mapping time
    rdfs:subClassOf skos:Concept ;
    rdfs:label "Load Capability"@en ;
    rdfs:comment "Abstract class representing track load capabilities, defined as a combination of the line category and speed at the weakest point of the track"@en .

era-gaugings:GaugingProfile a owl:Class ; # Concepts of this class are dynamically genereated at mapping time
    rdfs:subClassOf skos:Concept ;
    rdfs:label "Gauging Profile"@en ;
    rdfs:comment "Abstract class representing gauging profiles"@en .

era-tds:TrainDetectionSystem a owl:Class ; # Concepts of this class are dynamically genereated at mapping time
    rdfs:subClassOf skos:Concept ;
    rdfs:label "Train Detection System"@en ;
    rdfs:comment "Abstract class representing train detection systems"@en .

era-ftds:FrenchTrainDetectionSystemLimitation a owl:Class ;
    rdfs:subClassOf skos:Concept ;
    rdfs:label "French Train Detection System Limitation"@en ;
    rdfs:comment "Abstract class representing french train detection systems limitations"@en .

era-am:AxleBearingMonitoring a owl:Class ; # Concepts of this class are dynamically genereated at mapping time
    rdfs:subClassOf skos:Concept ;
    rdfs:label "Axle Bearing Condition Monitoring"@en ;
    rdfs:comment "Abstract class representing axle bearing condition monitoring setups"@en .

era-tc:ThermalCapacityTSIReference a owl:Class ; # Concepts of this class are dynamically genereated at mapping time
    rdfs:subClassOf skos:Concept ;
    rdfs:label "Thermal Capacity TSI Reference"@en ;
    rdfs:comment "Abstract class representing reference cases of TSI thermal capacities"@en .

era-ic:IceCondition a owl:Class ; # Concepts of this class are dynamically genereated at mapping time
    rdfs:subClassOf skos:Concept ;
    rdfs:label "Ice Condition"@en ;
    rdfs:comment "Abstract class representing ice, snow and hail conditions"@en .

era-cls:ContactLineSystem a owl:Class ; # Concepts of this class are dynamically genereated at mapping time
    rdfs:subClassOf skos:Concept ;
    rdfs:label "Contact Line System"@en ;
    rdfs:comment "Abstract class representing contact line systems"@en .

era-rs-fire:Category a owl:Class ;
    rdfs:subClassOf skos:Concept ;
    rdfs:label "Rolling Stock Fire Category"@en ;
    rdfs:comment "Abstract class representing fire categories of rolling stock. Rolling stock admitted in tunnels shall belong to either of the fire safety categories A and B"@en .

#################################################################
#
#    Data Types
#
#################################################################


#################################################################
#
#    Concepts
#
#################################################################


########## Vehicle categories ##########

era-vehicles:tractionVehicles a era-vehicles:Category ;
    skos:prefLabel "Traction Vehicles"@en .

era-vehicles:hauledPassenger a era-vehicles:Category ;
    skos:prefLabel "Hauled Passenger Vehicles"@en .

era-vehicles:freightWagons a era-vehicles:Category ;
    skos:prefLabel "Freight Wagons"@en .

era-vehicles:specialVehicles a era-vehicles:Category ;
    skos:prefLabel "Special Vehicles"@en .

########## Vehicle subcategories ##########

era-vehicles:locomotive a era-vehicles:SubCategory ;
    skos:broader era-vehicles:tractionVehicles ;
    skos:prefLabel "Locomotive"@en .

era-vehicles:passengerTrainset a era-vehicles:SubCategory ;
    skos:broader era-vehicles:tractionVehicles ;
    skos:prefLabel "Self-propelled passenger trainset (incl. railbusses)"@en .

era-vehicles:freightTrainset a era-vehicles:SubCategory ;
    skos:broader era-vehicles:tractionVehicles ;
    skos:prefLabel "Self-propelled freight trainset"@en .

era-vehicles:shunter a era-vehicles:SubCategory ;
    skos:broader era-vehicles:tractionVehicles ;
    skos:prefLabel "Shunter"@en .

era-vehicles:otherTractionVehicles a era-vehicles:SubCategory ;
    skos:broader era-vehicles:tractionVehicles ;
    skos:prefLabel "Other (tramways, light rail vehicles, etc)"@en .

era-vehicles:passengerCoach a era-vehicles:SubCategory ;
    skos:broader era-vehicles:hauledPassenger ;
    skos:prefLabel "Passenger Coach (incl. sleeping cars, restaurant, etc.)"@en .

era-vehicles:van a era-vehicles:SubCategory ;
    skos:broader era-vehicles:hauledPassenger ;
    skos:prefLabel "Van"@en .

era-vehicles:carCarrier a era-vehicles:SubCategory ;
    skos:broader era-vehicles:hauledPassenger ;
    skos:prefLabel "Car Carrier"@en .

era-vehicles:serviceVehicle a era-vehicles:SubCategory ;
    skos:broader era-vehicles:hauledPassenger ;
    skos:prefLabel "Vehicle for services (e.g. kitchen)"@en .

era-vehicles:coachesRake a era-vehicles:SubCategory ;
    skos:broader era-vehicles:hauledPassenger ;
    skos:prefLabel "Fixed rake of coaches"@en .

era-vehicles:otherHauledPassenger a era-vehicles:SubCategory ;
    skos:broader era-vehicles:hauledPassenger ;
    skos:prefLabel "Other hauled passenger vehicles"@en .

era-vehicles:freightWagon a era-vehicles:SubCategory ;
    skos:broader era-vehicles:freightWagons ;
    skos:prefLabel "Freight wagon"@en .

era-vehicles:freightWagonsRake a era-vehicles:SubCategory ;
    skos:broader era-vehicles:freightWagons ;
    skos:prefLabel "Fixed rake of freight wagons"@en .

era-vehicles:selfPropelledSpecialVehicle a era-vehicles:SubCategory ;
    skos:broader era-vehicles:specialVehicles ;
    skos:prefLabel "Self-propelled special vehicle"@en .

era-vehicles:hauledSpecialVehicle a era-vehicles:SubCategory ;
    skos:broader era-vehicles:specialVehicles ;
    skos:prefLabel "Hauled special vehicle"@en .


########## French train detection system limitations ##########

era-tds:N+1 a era-rs-fire:Category ;
    skos:prefLabel "N+1" ;
    skos:definition "Sections with tonnage circulated per track is inferior to 15000 tons/day/track"@en .

era-tds:N+2 a era-rs-fire:Category ;
    skos:prefLabel "N+2" ;
    skos:definition "Sections with directional Interlocking"@en .

era-tds:N+3 a era-rs-fire:Category ;
    skos:prefLabel "N+3" ;
    skos:definition "Sections with 45-second delay for directional interlocking"@en .

era-tds:N+4 a era-rs-fire:Category ;
    skos:prefLabel "N+4" ;
    skos:definition "Sections with Installation with track circuit announcement"@en .

era-tds:N+5 a era-rs-fire:Category ;
    skos:prefLabel "N+5" ;
    skos:definition "Sections with absence of a shunting assistance pedal in the normal direction of circulation for non-reversible double track lines"@en .

era-tds:N+6 a era-rs-fire:Category ;
    skos:prefLabel "N+6" ;
    skos:definition "Sections with absence of a shunting assistance pedal regardless of the direction of traffic for single track lines and tracks for two way working"@en .

era-tds:N+7 a era-rs-fire:Category ;
    skos:prefLabel "N+7" ;
    skos:definition "Sections with absence of a pedal announcement mechanism"@en .

era-tds:N+8 a era-rs-fire:Category ;
    skos:prefLabel "N+8" ;
    skos:definition "Sections with 45-second delay for specific announcement reset devices"@en .

########## Rolling stock fire categories ##########

era-rs-fire:a a era-rs-fire:Category ;
    skos:prefLabel "A" ;
    skos:definition "Rolling stock which is designed and built to operate on underground sections and tunnels of not more than 5 km in length, with side evacuation available is defined as category A"@en .

era-rs-fire:b a era-rs-fire:Category ;
    skos:prefLabel "B" ;
    skos:definition "Rolling stock which is designed and built to operate in all tunnels of the trans-European Network is defined as category B"@en .

era-rs-fire:none a era-rs-fire:Category ;
    skos:prefLabel "None"@en ;
    skos:definition "None of rolling stock fire categories A or B shall be applied on a tunnel"@en .